compiler/backend/proofs/source_to_sourceProofScript.sml
@@ -3,21 +3,26 @@
  *)
 Theory source_to_sourceProof
 Ancestors
-  source_letProof source_to_source evaluate evaluateProps
+  source_letProof source_dceProof source_to_source evaluate evaluateProps
   semanticPrimitives semanticPrimitivesProps misc[qualified]
-  semantics ast source_evalProof
+  semantics ast source_evalProof semanticsProps
 Libs
   preamble
 
 
 Theorem compile_semantics:
+  env.v = nsEmpty ∧
+  (∀x. s.eval_state = SOME x ⇒ ∃ev. x = EvalDecs ev) ∧
   ¬semantics_prog s env prog Fail ∧
   semantics_prog s env prog outcome ⇒
     semantics_prog s env (compile prog) outcome
 Proof
   rw [compile_def]
-  \\ irule source_letProofTheory.compile_semantics
-  \\ gs []
+  \\ drule_all source_dceProofTheory.compile_semantics \\ rw []
+  \\ irule source_letProofTheory.compile_semantics \\ rw []
+  \\ Cases_on ‘outcome = Fail’ \\ fs []
+  \\ CCONTR_TAC \\ gvs []
+  \\ imp_res_tac semantics_prog_deterministic
 QED
 
 Theorem compile_semantics_oracle:
@@ -26,12 +31,11 @@ Theorem compile_semantics_oracle:
   ¬ semantics_prog s env prog Fail ∧
   semantics_prog s env prog outcome ⇒
   semantics_prog (s with eval_state updated_by
-            source_evalProof$adjust_oracle ci (compile ∘ f))
+            source_evalProof$adjust_oracle ci (source_to_source$inc_compile ∘ f))
         env prog outcome
 Proof
-  rw [compile_def]
+  rw [compile_def,
+      SRULE [LET_THM, GSYM FUN_EQ_THM, SF ETA_ss] source_to_sourceTheory.inc_compile_def]
   \\ irule source_letProofTheory.compile_semantics_oracle
   \\ simp []
 QED
-
-
